feat(*) upgrade unification

Transport/Examples/Transport_PER.thy
@@ -4,9 +4,9 @@ theory Transport_PER
   imports
     Transport.Transport
     Transport_Rel_If
-    "HOL-Eisbach.Eisbach"
     ML_Unification.ML_Unification
     ML_Unification.ML_Unification_Resolution
+    Logging.ML_Attributes
   keywords "transport_term" :: thy_goal_defn
 begin
 
@@ -16,7 +16,7 @@ to work with equivalences on partial equivalence relations.
 It is also not forming the compositions of equivalences so far.
 The support for dependent function relators is restricted to the form
 described in
-@{thm transport_Dep_Fun_Rel_no_dep_fun.partial_equivalence_rel_equivalenceI}.
+@{thm transport_Dep_Fun_Rel_no_dep_fun.partial_equivalence_rel_equivalenceI}:
 The relations can be dependent, but the functions must be simple.
 This is not production ready, but a proof of concept.
 
@@ -31,17 +31,17 @@ begin
 
 lemma left_Galois_left_if_left_rel_if_partial_equivalence_rel_equivalence:
   assumes "((\<le>\<^bsub>L\<^esub>) \<equiv>\<^bsub>PER\<^esub> (\<le>\<^bsub>R\<^esub>)) l r"
-  and "x \<le>\<^bsub>L\<^esub> x"
+  and "x \<le>\<^bsub>L\<^esub> x'"
   shows "x \<^bsub>L\<^esub>\<lessapprox> l x"
   using assms by (intro left_Galois_left_if_left_rel_if_inflationary_on_in_fieldI)
   (blast elim: preorder_equivalence_order_equivalenceE)+
 
 definition "transport_per x y \<equiv> ((\<le>\<^bsub>L\<^esub>) \<equiv>\<^bsub>PER\<^esub> (\<le>\<^bsub>R\<^esub>)) l r \<and> x \<^bsub>L\<^esub>\<lessapprox> y"
 
-text \<open>The choice of @{term "x \<le>\<^bsub>L\<^esub> x"} is arbitrary. All we need is @{term "in_dom (\<le>\<^bsub>L\<^esub>) x"}.\<close>
+text \<open>The choice of @{term "x'"} is arbitrary. All we need is @{term "in_dom (\<le>\<^bsub>L\<^esub>) x"}.\<close>
 lemma transport_per_start:
   assumes "((\<le>\<^bsub>L\<^esub>) \<equiv>\<^bsub>PER\<^esub> (\<le>\<^bsub>R\<^esub>)) l r"
-  and "x \<le>\<^bsub>L\<^esub> x"
+  and "x \<le>\<^bsub>L\<^esub> x'"
   shows "transport_per x (l x)"
   using assms unfolding transport_per_def
   by (blast intro: left_Galois_left_if_left_rel_if_partial_equivalence_rel_equivalence)
@@ -90,10 +90,11 @@ qed
 
 end
 
-ML_file\<open>util.ML\<close>
-ML_file\<open>parse_util.ML\<close>
+ML_file\<open>transport_util.ML\<close>
+ML_file\<open>transport_parse_util.ML\<close>
 
 ML\<open>
+  structure Norm = Normalisation
   structure Util = Transport_Util
   structure CUtil = Conversion_Util
   structure UUtil = Unification_Util
@@ -101,20 +102,19 @@ ML\<open>
 \<close>
 
 ML\<open>
+  (* val simp_rhs *)
+  val simp_rhs = Simplifier.rewrite #> CUtil.rhs_conv #> CUtil.thm_conv
+
   (*simplifies the generated definition of a transported term*)
-  fun simp_def ctxt simps y_def =
+  fun simp_transported_def ctxt simps y_def =
     let
       val ctxt = ctxt addsimps simps
-      val rhs_simp_conv = Simplifier.rewrite ctxt |> CUtil.rhs_conv |> CUtil.thm_conv
-      val y_def_simplified = rhs_simp_conv y_def
-
       val y_def_eta_expanded = Util.equality_eta_expand ctxt "x" y_def
-      val y_def_eta_expanded_simplified = rhs_simp_conv y_def_eta_expanded
-    in (y_def_simplified, y_def_eta_expanded_simplified) end
+    in apply2 (simp_rhs ctxt) (y_def, y_def_eta_expanded) end
 \<close>
 
-text \<open>Definitions used by Transport that need to be folded before a proof and
-unfolded after success.\<close>
+text \<open>Definitions used by Transport that need to be folded before a PER proof
+and unfolded after success.\<close>
 ML\<open>
   structure Transport_Defs = Named_Thms(
     val name = @{binding "transport_def"}
@@ -129,24 +129,33 @@ declare
 
 ML\<open>
   (*first-order unification with higher-order pattern unification with hints as a fallback*)
-  val norm_thm_beta_eta =
-    UUtil.norm_thm_beta_eta UUtil.norm_type_unif UUtil.norm_term_unif
-  fun unify_hints ctxt =
+  val norm_thm_beta_eta = Norm.beta_eta_norm_thm Norm.norm_type_unif Norm.norm_term_unif
+  fun unify_hints binders ctxt =
     let
       val unify_types = UUtil.unify_types
-      val hints = Unification_Hints.gen_hint_list ctxt
+      val hints = Unification_Hints.get_hints ctxt
       val unif_hints = Higher_Order_Pattern_Unification.unify
+      val norm_term_unif = Norm.norm_term_unif
       val norm_thm_unif = norm_thm_beta_eta
       fun ho_unify ctxt = Higher_Order_Pattern_Unification.e_unify
-        unify_types (Unification_Hints.try_hints unif_hints norm_thm_unif ho_unify hints)
+        unify_types (Unification_Hints.try_hints unif_hints norm_term_unif norm_thm_unif ho_unify hints)
         ctxt
       val unify = First_Order_Unification.e_unify unify_types ho_unify
-    in unify ctxt end
+    in unify binders ctxt end
 
   (*resoluton with above unifier*)
-  val any_unify_hints_resolve_tac = Unify_Resolve.any_unify_resolve_tac
+  val any_unify_hints_resolve_tac =
+    (* Unify_Resolve.any_unify_resolve_tac *)
+    Unify_Resolve.no_lift_any_unify_resolve_tac
     norm_thm_beta_eta unify_hints
+
+  fun get_theorems_tac f get_theorems ctxt = f (get_theorems ctxt) ctxt
+  val get_theorems_resolve_tac = get_theorems_tac any_unify_hints_resolve_tac
 \<close>
+
+method_setup resolve_hints =
+  \<open>Attrib.thms >> (SIMPLE_METHOD' oo any_unify_hints_resolve_tac)\<close>
+  "Resolution with unification hints"
 
 text \<open>Introduction rules for the PER equivalence prover.\<close>
 ML\<open>
@@ -158,56 +167,60 @@ ML\<open>
 \<close>
 
 declare
-  (*completely dependent case not supported as of now*)
+  (*dependent case currently disabled by default since they easily make the
+    unifier enumerate many undesired instantiations*)
   (* transport_Dep_Fun_Rel.partial_equivalence_rel_equivalenceI[per_intro] *)
-  transport_Dep_Fun_Rel_no_dep_fun.partial_equivalence_rel_equivalenceI[per_intro]
-  (*transport.rel_if_partial_equivalence_rel_equivalence_if_iff_if_partial_equivalence_rel_equivalenceI[per_intro]*)
-  transport_Fun_Rel.partial_equivalence_rel_equivalenceI[per_intro]
+  (* transport.rel_if_partial_equivalence_rel_equivalence_if_iff_if_partial_equivalence_rel_equivalenceI[rotated, per_intro]
+  transport_Dep_Fun_Rel_no_dep_fun.partial_equivalence_rel_equivalenceI
+    [ML_rattr \<open>Conversion_Util.move_prems_to_front_conv [1] |> CUtil.thm_conv |> K\<close>,
+    ML_rattr \<open>Conversion_Util.move_prems_to_front_conv [2,3] |> CUtil.thm_conv |> K\<close>,
+    per_intro] *)
+  transport_Fun_Rel.partial_equivalence_rel_equivalenceI[rotated, per_intro]
   transport_eq_id.partial_equivalence_rel_equivalenceI[per_intro]
   transport_eq_restrict_id.partial_equivalence_rel_equivalence[per_intro]
 
 ML\<open>
-  fun per_prover_tac ctxt =
-    let
-      val per_intros = PER_Intros.get ctxt
-      val resolve_tac = any_unify_hints_resolve_tac
-    in REPEAT1 o resolve_tac per_intros ctxt end
+  fun per_prover_tac ctxt = REPEAT_ALL_NEW (get_theorems_resolve_tac PER_Intros.get ctxt)
 \<close>
 
 method_setup per_prover =
-  \<open>Scan.succeed (SIMPLE_METHOD o HEADGOAL o per_prover_tac)\<close>
+  \<open>Scan.succeed (SIMPLE_METHOD' o per_prover_tac)\<close>
   "PER prover for Transport"
 
 ML\<open>
-  structure Transport_Parametrics = Named_Thms(
-    val name = @{binding "transport_parametric"}
-    val description = "Parametricity theorems for Transport"
+  structure Transport_in_dom = Named_Thms(
+    val name = @{binding "transport_in_dom"}
+    val description = "In domain theorems for Transport"
   )
-  val _ = Theory.setup Transport_Parametrics.setup
+  val _ = Theory.setup Transport_in_dom.setup
 \<close>
 
-text \<open>Discharges the @{term "L x x"} goals by registered lemmas.\<close>
+text \<open>Discharges the @{term "L x x'"} goals by registered lemmas.\<close>
 ML\<open>
-  fun parametricity_prover_tac ctxt =
-    let
-      val transport_defs = Transport_Defs.get ctxt
-      val transport_parametric = Transport_Parametrics.get ctxt
-      val resolve_tac = any_unify_hints_resolve_tac
-      val ctxt = clear_simpset ctxt addsimps transport_defs
-    in
-      full_simp_tac ctxt
-      THEN' resolve_tac transport_parametric ctxt
-    end
+  fun transport_in_dom_prover_tac ctxt = get_theorems_resolve_tac Transport_in_dom.get ctxt
 \<close>
 
-method_setup parametricity_prover =
-  \<open>Scan.succeed (SIMPLE_METHOD o FIRSTGOAL o parametricity_prover_tac)\<close>
+method_setup transport_in_dom_prover =
+  \<open>Scan.succeed (SIMPLE_METHOD' o transport_in_dom_prover_tac)\<close>
   "parametricity prover for Transport"
 
+text \<open>Blackbox prover: first derive the PER equivalence, then look for registered domain lemmas.\<close>
+ML\<open>
+  fun unfold_tac thms ctxt = simp_tac (clear_simpset ctxt addsimps thms)
+  val unfold_transport_defs_tac = get_theorems_tac unfold_tac Transport_Defs.get
 
-text \<open>First derive the PER equivalence, then look for registered
-parametricity lemmas.\<close>
-method transport_term_prover = per_prover, parametricity_prover?
+  fun transport_prover ctxt i =
+    per_prover_tac ctxt i
+    THEN TRY (SOMEGOAL
+      (TRY o unfold_transport_defs_tac ctxt
+      THEN' transport_in_dom_prover_tac ctxt)
+    )
+\<close>
+
+method_setup transport_prover =
+  \<open>Scan.succeed (SIMPLE_METHOD' o transport_prover)\<close>
+  "Blackbox prover for Transport"
+
 
 ML\<open>
   structure Transport_Related_Intros = Named_Thms(
@@ -227,31 +240,39 @@ ML\<open>
 \<close>
 
 declare
-  transport_Fun_Rel.left_Galois_eq_Fun_Rel_left_Galois[transport_relator_rewrite]
   transport_id.left_Galois_eq_left[transport_relator_rewrite]
+  transport_Fun_Rel.left_Galois_eq_Fun_Rel_left_Galois[transport_relator_rewrite]
 
 ML\<open>
+  fun fold_tac thms =
+    Tactic_Util.FOCUS_PARAMS_CTXT
+      (fn ctxt => PRIMITIVE (Raw_Simplifier.fold_rule (clear_simpset ctxt) thms))
+
   (*simple rewrite tactic for Galois relators*)
   fun per_simp_prover ctxt thm =
     let
       val prems = Thm.cprems_of thm
       val per_prover_tac = per_prover_tac ctxt
-      fun prove_prem prem =
-        Goal.prove_internal ctxt [] prem (fn _ => HEADGOAL per_prover_tac)
-    in
-      try (map prove_prem) prems
-      |> Option.map (curry (op OF) thm)
-    end
+      fun prove_prem prem = Goal.prove_internal ctxt [] prem (fn _ => HEADGOAL per_prover_tac)
+    in try (map prove_prem) prems |> Option.map (curry (op OF) thm) end
   fun transport_relator_rewrite ctxt thm =
     let
       val transport_defs = Transport_Defs.get ctxt
-      val thm = Local_Defs.fold ctxt transport_defs thm
       val transport_relator_rewrites = Transport_Relator_Rewrites.get ctxt
       val ctxt = (clear_simpset ctxt) addsimps transport_relator_rewrites
     in
-      Raw_Simplifier.rewrite_thm (false, false, false) per_simp_prover ctxt thm
+      Local_Defs.fold ctxt transport_defs thm
+      |> Raw_Simplifier.rewrite_thm (false, false, false) per_simp_prover ctxt
     end
+  fun transport_relator_rewrite_tac ctxt =
+    EqSubst.eqsubst_tac ctxt [0] (Transport_Relator_Rewrites.get ctxt)
+    THEN_ALL_NEW TRY o SOLVED' (per_prover_tac ctxt)
 \<close>
+
+method_setup transport_relator_rewrite =
+  \<open>Scan.succeed (SIMPLE_METHOD' o transport_relator_rewrite_tac)\<close>
+  "Rewrite Transport relator"
+
 
 text \<open>Parsing setup\<close>
 
@@ -313,7 +334,7 @@ ML\<open>
   (*bindings for generated theorems and definitions*)
   val binding_transport_per = \<^binding>\<open>transport_per\<close>
   val binding_per = \<^binding>\<open>per\<close>
-  val binding_parametric = \<^binding>\<open>parametric\<close>
+  val binding_in_dom = \<^binding>\<open>in_dom\<close>
   val binding_related = \<^binding>\<open>related\<close>
   val binding_related_rewritten = \<^binding>\<open>related'\<close>
   val binding_def_simplified = \<^binding>\<open>eq\<close>
@@ -324,15 +345,15 @@ ML\<open>
       val ((_, (_, y_def)), ctxt) =
         Util.create_local_theory_def (binding, mixfix) [] y ctxt
       (*create simplified definition theorems*)
-      val def_simps = Transport_Defs.get ctxt
+      val transport_defs = Transport_Defs.get ctxt
       val (y_def_simplified, y_def_eta_expanded_simplified) =
-        simp_def ctxt def_simps y_def
+        simp_transported_def ctxt transport_defs y_def
       (*create relatedness theorems*)
       val related_thm_rewritten = transport_relator_rewrite ctxt related_thm
       fun prepare_fact (suffix, thm, attribs) =
         let
           val binding = (Util.add_suffix binding suffix, [])
-          val ctxt = (clear_simpset ctxt) addsimps def_simps
+          val ctxt = (clear_simpset ctxt) addsimps transport_defs
           val folded_thm =
             (*fold definition of transported term*)
             Local_Defs.fold ctxt [y_def] thm
@@ -350,7 +371,7 @@ ML\<open>
     in Local_Theory.notes facts ctxt |> snd end
 
   (*black-box transport as described in the Transport paper*)
-  fun after_qed_blackbox (binding, mixfix) [thms as [per_thm, parametricity_thm]] ctxt =
+  fun after_qed_blackbox (binding, mixfix) [thms as [per_thm, in_dom_thm]] ctxt =
     let
       val transport_per_thm = List.foldl (op INCR_COMP) transport_per_start_thm thms
       (*fix possibly occurring meta type variables*)
@@ -361,8 +382,8 @@ ML\<open>
       val binding_thms = [
           (binding_transport_per, transport_per_thm, []),
           (binding_per, per_thm, []),
-          (binding_parametric, parametricity_thm,
-            [Util.attrib_to_src Transport_Parametrics.add])
+          (binding_in_dom, in_dom_thm,
+            [Util.attrib_to_src Transport_in_dom.add])
         ]
     in note_facts (binding, mixfix) ctxt related_thm y binding_thms end
 
@@ -423,7 +444,7 @@ ML\<open>
           val opts = [optL, optR, opty]
           val opts_default_names = ["L", "R", "y"]
           val opts_constraints =
-            [Util.mk_rel_type (Thm.typ_of_cterm cx), Util.mk_rel_type yT, yT]
+            [Util.mk_hom_rel_type (Thm.typ_of_cterm cx), Util.mk_hom_rel_type yT, yT]
             |> map Type.constraint
           (***parse***)
           val opts = map (Syntax.parse_term ctxt |> Option.map) opts
@@ -462,22 +483,91 @@ ML\<open>
       "transport of definition" (parse_strings >> setup_proof)
 \<close>
 
-text \<open>The following sets up an experimental white-box prover; but it
-can be ignored as it is not very functional at the moment.\<close>
-lemmas Fun_Rel_relD = Dep_Fun_Rel_relD[where ?S="\<lambda>_ _. S" for S]
-declare Fun_Rel_relD[transport_related_intro]
+text \<open>The following sets up an experimental white-box prover.\<close>
+lemmas related_Fun_Rel_combI = Dep_Fun_Rel_relD[where ?S="\<lambda>_ _. S" for S, rotated]
+lemma related_Fun_Rel_lambdaI:
+  assumes "\<And>x y. R x y \<Longrightarrow> S (f x) (g y)"
+  and "T = (R \<Rrightarrow> S)"
+  shows "T f g"
+  using assms by blast
 
 ML\<open>
-  fun transport_related_tac ctxt =
+  fun mk_transport_related_tac cc_comb cc_lambda ctxt =
     let
       val transport_related_intros = Transport_Related_Intros.get ctxt
-      val resolve_tac = any_unify_hints_resolve_tac
-    in REPEAT1 o resolve_tac transport_related_intros ctxt end
+      val related_tac = any_unify_hints_resolve_tac transport_related_intros ctxt
+      val assume_tac = assume_tac ctxt
+      val comb_tac = any_unify_hints_resolve_tac @{thms related_Fun_Rel_combI} ctxt
+      val lambda_tac = any_unify_hints_resolve_tac @{thms related_Fun_Rel_lambdaI} ctxt
+    in
+      Tactic_Util.CONCAT' [
+        related_tac,
+        cc_comb comb_tac,
+        cc_lambda lambda_tac,
+        assume_tac
+      ]
+    end
+  val transport_related_step_tac =
+    let fun cc_comb tac i = tac i
+      THEN prefer_tac i
+      THEN prefer_tac (i + 1)
+    in mk_transport_related_tac cc_comb I end
+  fun transport_related_tac ctxt =
+    let
+      fun transport_related_tac cc =
+        let
+          fun cc_comb tac = tac THEN_ALL_NEW TRY o cc
+          fun cc_lambda tac = tac THEN' TRY o cc
+        in mk_transport_related_tac cc_comb cc_lambda ctxt end
+      fun fix tac i thm = tac (fix tac) i thm
+    in fix transport_related_tac end
 \<close>
 
 method_setup transport_related_prover =
-  \<open>Scan.succeed (SIMPLE_METHOD o REPEAT_SOME o transport_related_tac)\<close>
+  \<open>Scan.succeed (SIMPLE_METHOD' o transport_related_tac)\<close>
   "Relatedness prover for Transport"
+
+ML\<open>
+  fun instantiate_tac name ct ctxt =
+    PRIMITIVE (Drule.infer_instantiate_types ctxt [((name, Thm.typ_of_cterm ct), ct)])
+    |> CHANGED
+
+  val map_dummyT = Term.map_types (K dummyT)
+
+  fun mk_term_skeleton maxidx t =
+    let
+      val consts = Term.add_consts t []
+      val (vars, _) = fold_map (uncurry UUtil.fresh_var o apfst Long_Name.base_name) consts maxidx
+      val t' = Term.subst_atomic (map2 (pair o Const) consts vars) t
+    in t' end
+
+  fun instantiate_skeleton_tac ctxt =
+    let fun tac ct =
+      let
+        val (x, y) = Util.cdest_judgement ct |> Thm.dest_binop
+        val skeleton =
+          mk_term_skeleton (Thm.maxidx_of_cterm ct) (Thm.term_of x)
+          |> map_dummyT
+          |> Type.constraint (Thm.typ_of_cterm y)
+          |> Syntax.check_term (Util.set_proof_mode_pattern ctxt)
+          |> Thm.cterm_of ctxt
+      in instantiate_tac (Thm.term_of y |> dest_Var |> fst) skeleton ctxt end
+    in Tactic_Util.CSUBGOAL_DATA I (K o tac) end
+\<close>
+
+ML\<open>
+  fun transport_whitebox_tac ctxt =
+    instantiate_skeleton_tac ctxt
+    THEN' transport_related_tac ctxt
+    THEN_ALL_NEW (
+      TRY o REPEAT1 o transport_relator_rewrite_tac ctxt
+      THEN' TRY o any_unify_hints_resolve_tac @{thms refl} ctxt
+    )
+\<close>
+
+method_setup transport_whitebox_prover =
+  \<open>Scan.succeed (SIMPLE_METHOD' o transport_whitebox_tac)\<close>
+  "Whitebox prover for Transport"
 
 
 end
