Transport/Examples/Transport_Set_Extension.thy
@@ -5,6 +5,7 @@ theory Transport_Set_Extension
     Isabelle_Set.Integers
     Transport_PER
     Transport_Syntax
+    Logging.ML_Attributes
 begin
 
 paragraph \<open>Summary\<close>
@@ -26,73 +27,87 @@ text \<open>Proof of equivalence is done for all set-extensions in
 @{theory Isabelle_Set.Set_Extensions_Transport}.\<close>
 declare Int.partial_equivalence_rel_equivalence[per_intro]
 
-definition "int_repZ ir i \<equiv> i \<in> \<int> \<and> ir = Int.r i"
+definition "RepZ ir i \<equiv> i \<in> \<int> \<and> ir = Int.r i"
 
-lemma int_rep_Galois_eq_int_repZ: "(\<^bsub>(=\<^bsub>int_rep\<^esub>)\<^esub>\<lessapprox>\<^bsub>(=\<^bsub>\<int>\<^esub>) Int.r\<^esub>) \<equiv> int_repZ"
-  unfolding galois_rel.Galois_def int_repZ_def by (intro eq_reflection ext) auto
+lemma int_rep_Galois_eq_RepZ: "(\<^bsub>(=\<^bsub>int_rep\<^esub>)\<^esub>\<lessapprox>\<^bsub>(=\<^bsub>\<int>\<^esub>) Int.r\<^esub>) \<equiv> RepZ"
+  unfolding galois_rel.Galois_def RepZ_def by (intro eq_reflection ext) auto
 
-declare int_rep_Galois_eq_int_repZ[transport_relator_rewrite, unif_hint]
+declare int_rep_Galois_eq_RepZ[transport_relator_rewrite, unif_hint]
 
 text \<open>Transport from natural numbers into non-negative integers.\<close>
 
-lemma Int_Rep_nonneg_parametric [transport_parametric]:
+lemma Int_Rep_nonneg_parametric [transport_in_dom]:
   "((=\<^bsub>\<nat>\<^esub>) \<Rrightarrow> Int.L) Int_Rep_nonneg Int_Rep_nonneg"
-  (*TODO: in the future, this should be provable without unfolding the definition
-  using just the soft-type of Int_Rep @{thm "Int_Rep_nonneg_type"}*)
   unfolding Int_Rep_nonneg_def int_rep_def by (intro Dep_Fun_Rel_relI) auto
 
 transport_term int_nonneg :: "set \<Rightarrow> set" where
   x = Int_Rep_nonneg and L = "(=\<^bsub>\<nat>\<^esub>) \<Rrightarrow> Int.L" and R = "((=\<^bsub>\<nat>\<^esub>) :: set \<Rightarrow> _) \<Rrightarrow> Int.R"
-  by transport_term_prover
+  by transport_prover
 
 text \<open>Transport from natural numbers into negative integers.\<close>
 
-lemma Int_Rep_neg_parametric [transport_parametric]:
+lemma Int_Rep_neg_parametric [transport_in_dom]:
   "((=\<^bsub>\<nat> \<setminus> {0}\<^esub>) \<Rrightarrow> Int.L) Int_Rep_neg Int_Rep_neg"
   unfolding Int_Rep_neg_def int_rep_def by (intro Dep_Fun_Rel_relI) auto
 
 transport_term int_neg
   where x = Int_Rep_neg and L = "(=\<^bsub>\<nat> \<setminus> {0}\<^esub>) \<Rrightarrow> Int.L"
   and R = "((=\<^bsub>\<nat> \<setminus> {0}\<^esub>) :: set \<Rightarrow> _) \<Rrightarrow> Int.R"
-  by transport_term_prover
+  by transport_prover
 
 text \<open>Transport 0.\<close>
 
-lemma Int_Rep_zero_parametric [transport_parametric]: "Int_Rep_zero =\<^bsub>int_rep\<^esub> Int_Rep_zero"
+lemma Int_Rep_zero_parametric [transport_in_dom]: "Int_Rep_zero =\<^bsub>int_rep\<^esub> Int_Rep_zero"
   by auto
 
 transport_term int_zero where x = Int_Rep_zero and L = Int.L and R = Int.R
-  by transport_term_prover
+  by transport_prover
 
 text \<open>There is some very limited white-box transport support in the prototype.\<close>
-
- transport_term int_zero' where x = Int_Rep_zero and L = Int.L and R = Int.R
+transport_term int_zero' where x = Int_Rep_zero and L = Int.L and R = Int.R
   unfold Int_Rep_zero_def ! (*invoking "!" opens the whitebox goal*)
-  by transport_related_prover (*the whitebox transport prover*)
-  auto
+  (*the whitebox transport prover*)
+  by transport_whitebox_prover auto
 
 text \<open>Note the difference in definition between the blackbox and whitebox term\<close>
 print_statement int_zero_def int_zero'_def
 
+transport_term lambdatest :: "'a \<Rightarrow> set" where x = "\<lambda>(_ :: 'a). Int_Rep_zero"
+  ! (*invoking "!" opens the whitebox goal*)
+  (*the whitebox transport prover*)
+  by transport_whitebox_prover
+
+transport_term apptest :: "set" where x = "Int_Rep_nonneg 0" !
+  by transport_whitebox_prover auto
+
 text \<open>Transport addition\<close>
 
-lemma Int_Rep_add_parametric [transport_parametric]:
+lemma Int_Rep_add_parametric [transport_in_dom]:
   "(Int.L \<Rrightarrow> Int.L \<Rrightarrow> Int.L) Int_Rep_add Int_Rep_add"
   by (intro Dep_Fun_Rel_relI) fastforce
 
 transport_term int_add where x = Int_Rep_add
   and L = "Int.L \<Rrightarrow> Int.L \<Rrightarrow> Int.L" and R = "Int.R \<Rrightarrow> Int.R \<Rrightarrow> Int.R"
-  by transport_term_prover
+  by transport_prover
 
 text \<open>Transport subtraction\<close>
 
-lemma Int_Rep_sub_parametric [transport_parametric]:
+lemma Int_Rep_sub_parametric [transport_in_dom]:
   "(Int.L \<Rrightarrow> Int.L \<Rrightarrow> Int.L) Int_Rep_sub Int_Rep_sub"
   by (intro Dep_Fun_Rel_relI) fastforce
 
 transport_term int_sub where x = Int_Rep_sub
   and L = "Int.L \<Rrightarrow> Int.L \<Rrightarrow> Int.L" and R = "Int.R \<Rrightarrow> Int.R \<Rrightarrow> Int.R"
-  by transport_term_prover
+  by transport_prover
+
+
+(* declare[[ML_dattr "fn _ => Logger.set_log_levels First_Order_Unification.logger Logger.ALL"]] *)
+(* declare[[show_types]] *)
+(* declare[[ML_dattr "fn _ => Logger.set_log_levels Higher_Order_Pattern_Unification.logger Logger.DEBUG"]] *)
+(* declare[[ML_dattr "fn _ => Logger.map_logger Higher_Order_Pattern_Unification.logger
+  (Logger.set_config_output (K writeln) |> Option.map)"]] *)
+transport_term abc :: "set \<Rightarrow> set \<Rightarrow> set" where x = "\<lambda>(_ :: set) y. Int_Rep_add y y" !
+  by transport_whitebox_prover
 
 text \<open>Transport a higher-order function\<close>
 
@@ -101,30 +116,28 @@ definition "Int_Rep_if P i x y \<equiv> if P i then x else y"
 lemma "Int_Rep_if : (Int_Rep \<Rightarrow> Bool) \<Rightarrow> Int_Rep \<Rightarrow> A \<Rightarrow> A \<Rightarrow> A"
   unfolding Int_Rep_if_def by discharge_types
 
-lemma Int_Rep_if_parametric [transport_parametric]:
+lemma Int_Rep_if_parametric [transport_in_dom]:
   "((Int.L \<Rrightarrow> (\<longleftrightarrow>)) \<Rrightarrow> Int.L \<Rrightarrow> (=)) Int_Rep_if Int_Rep_if"
   unfolding Int_Rep_if_def by (intro Dep_Fun_Rel_relI) auto
 
 transport_term int_if :: "(set \<Rightarrow> bool) \<Rightarrow> set \<Rightarrow> 'a \<Rightarrow> 'a \<Rightarrow> 'a"
   where x = "Int_Rep_if :: (set \<Rightarrow> bool) \<Rightarrow> set \<Rightarrow> 'a \<Rightarrow> 'a \<Rightarrow> 'a"
   and L = "(Int.L \<Rrightarrow> (\<longleftrightarrow>)) \<Rrightarrow> Int.L \<Rrightarrow> (=)"
-  by transport_term_prover
+  by transport_prover
 
 lemma Galois_id_hint [unif_hint]:
   "(L :: 'a \<Rightarrow> 'a \<Rightarrow> bool) \<equiv> R \<Longrightarrow> r \<equiv> id \<Longrightarrow> E \<equiv> L \<Longrightarrow> (\<^bsub>L\<^esub>\<lessapprox>\<^bsub>R r\<^esub>) \<equiv> E"
   by (simp only: eq_reflection[OF transport_id.left_Galois_eq_left])
 
 context
-  fixes P P' :: "set \<Rightarrow> bool"
-  assumes Prel: "(int_repZ \<Rrightarrow> (=)) P P'"
+  fixes P :: "set \<Rightarrow> bool"
+  assumes [transport_related_intro]: "(RepZ \<Rrightarrow> (=)) P P"
 begin
 
 (*whitebox transport*)
 transport_term int_if_app_zero :: "'a \<Rightarrow> 'a \<Rightarrow> 'a"
   where x = "Int_Rep_if P Int_Rep_zero :: 'a \<Rightarrow> 'a \<Rightarrow> 'a" !
-  by transport_related_prover (fact Prel)
-
-thm int_if_app_zero_def
+  by transport_whitebox_prover
 
 end
 
@@ -134,7 +147,7 @@ lemma app_eq_Int_Rep_zero_type:
   "app_eq_Int_Rep_zero : (A \<Rightarrow> Int_Rep) \<Rightarrow> A \<Rightarrow> Bool"
   by discharge_types
 
-lemma app_eq_Int_Rep_parametric [transport_parametric]:
+lemma app_eq_Int_Rep_parametric [transport_in_dom]:
   "((R \<Rrightarrow> Int.L) \<Rrightarrow> R \<Rrightarrow> (\<longleftrightarrow>)) app_eq_Int_Rep_zero app_eq_Int_Rep_zero"
   unfolding app_eq_Int_Rep_zero_def
   by (intro Dep_Fun_Rel_relI) (auto elim!: eq_restrictE)
@@ -143,61 +156,60 @@ transport_term app_eq_int_zero
   where x = "app_eq_Int_Rep_zero :: (set \<Rightarrow> set) \<Rightarrow> _"
   and L = "(Int.L \<Rrightarrow> Int.L) \<Rrightarrow> Int.L \<Rrightarrow> (\<longleftrightarrow>)"
   and R = "(Int.R \<Rrightarrow> Int.R) \<Rrightarrow> Int.R \<Rrightarrow> (\<longleftrightarrow>)"
-  by transport_term_prover
+  by transport_prover
 
-lemma If_parametric [transport_parametric]: "((\<longleftrightarrow>) \<Rrightarrow> R \<Rrightarrow> R \<Rrightarrow> R) If If"
+lemma If_parametric [transport_in_dom, transport_related_intro]: "((\<longleftrightarrow>) \<Rrightarrow> R \<Rrightarrow> R \<Rrightarrow> R) If If"
   by (intro Dep_Fun_Rel_relI) auto
 
-lemma eq_parametric [transport_parametric]: "((=) \<Rrightarrow> (=) \<Rrightarrow> (\<longleftrightarrow>)) (=) (=)"
+lemma eq_parametric [transport_in_dom, transport_related_intro]:
+  (* "((=) \<Rrightarrow> (=) \<Rrightarrow> (\<longleftrightarrow>)) (=) (=)" *)
+  (* by (intro Dep_Fun_Rel_relI) auto *)
+  "(RepZ \<Rrightarrow> RepZ \<Rrightarrow> (\<longleftrightarrow>)) (=) (=)"
+  sorry
+
+lemma id_parametric [transport_in_dom, transport_related_intro]: "(R \<Rrightarrow> R) id id"
   by (intro Dep_Fun_Rel_relI) auto
 
-lemma id_parametric [transport_parametric]: "(R \<Rrightarrow> R) id id"
-  by (intro Dep_Fun_Rel_relI) auto
+context
+  fixes f :: "set \<Rightarrow> set"
+  assumes [transport_related_intro]: "(RepZ \<Rrightarrow> RepZ) f f"
+begin
 
-transport_term test_whitebox
+transport_term whitebox_if_app
   where x = "app_eq_Int_Rep_zero f Int_Rep_zero"
   and L = "(\<longleftrightarrow>)" and R = "(\<longleftrightarrow>)"
   unfold app_eq_Int_Rep_zero_def !
-  apply transport_related_prover
-  apply (tactic \<open>TRYALL (any_unify_hints_resolve_tac
-    (@{thm refl} :: @{thms transport_parametric}) @{context})\<close>)
-  oops
-
-lemma lambda_related:
-  assumes "\<And>x y. R x y \<Longrightarrow> S (f x) (g y)"
-  and "T = (R \<Rrightarrow> S)"
-  shows "T (\<lambda>x. f x) (\<lambda>y. g y)"
-  using assms by blast
-
-(* config[First_Order_Unification.Logger.log_level=10000] *)
-(* config[Unification_Hints.Logger.log_level=10000] *)
-(* config[Higher_Order_Pattern_Unification.Logger.log_level=10000] *)
-(* config[Unify_Resolve.Logger.log_level=10000] *)
-
-(* declare[[eta_contract=false]] *)
-(* declare[[show_types=true]] *)
+  by transport_whitebox_prover
 
 transport_term int_to_bool'
   where x = "app_eq_Int_Rep_zero :: (set \<Rightarrow> set) \<Rightarrow> _"
   and L = "(Int.L \<Rrightarrow> Int.L) \<Rrightarrow> Int.L \<Rrightarrow> (\<longleftrightarrow>)"
   and R = "(Int.R \<Rrightarrow> Int.R) \<Rrightarrow> Int.R \<Rrightarrow> (\<longleftrightarrow>)"
-  and y = "(\<lambda>g y. if g y = ?zero then ?True else ?False) ::(set \<Rightarrow> set) \<Rightarrow> set \<Rightarrow> bool"
   unfold app_eq_Int_Rep_zero_def !
-  apply (tactic \<open>any_unify_hints_resolve_tac @{context} [@{thm lambda_related}] 1\<close>)+
-  apply (tactic \<open>HEADGOAL (any_unify_hints_resolve_tac @{context}
-    @{thms transport_related_intro})\<close>)+
-  apply (tactic \<open>any_unify_hints_resolve_tac @{context} @{thms If_parametric} 1\<close>)+
-  apply (tactic \<open>any_unify_hints_resolve_tac @{context} @{thms transport_related_intro} 1\<close>)+
-  defer
-  apply (tactic \<open>any_unify_hints_resolve_tac @{context} @{thms transport_related_intro} 1\<close>)+
-  defer
-  defer
-  apply (tactic \<open>any_unify_hints_resolve_tac @{context} @{thms int_zero_related'} 1\<close>)
-  apply (tactic \<open>any_unify_hints_resolve_tac @{context}
-    (@{thms transport_parametric} @ [@{thm refl}]) 1\<close>)+
-  oops
+  apply (tactic \<open>instantiate_skeleton_tac @{context} 1\<close>)
+  apply (tactic \<open>transport_related_step_tac @{context} 1\<close>)
+  apply (tactic \<open>transport_related_step_tac @{context} 1\<close>)
+  apply (tactic \<open>transport_related_step_tac @{context} 1\<close>)
+  apply (tactic \<open>transport_related_step_tac @{context} 1\<close>)
+  apply (tactic \<open>transport_related_step_tac @{context} 1\<close>)
+  apply (tactic \<open>transport_related_step_tac @{context} 1\<close>)
+  apply (tactic \<open>transport_related_step_tac @{context} 1\<close>)
+  apply (tactic \<open>transport_related_step_tac @{context} 1\<close>)
+  apply (tactic \<open>transport_related_step_tac @{context} 1\<close>)
+  apply (tactic \<open>transport_related_step_tac @{context} 1\<close>)
+  apply assumption
+  apply (tactic \<open>transport_related_step_tac @{context} 1\<close>)
+  apply (tactic \<open>transport_related_step_tac @{context} 1\<close>)
+  apply (resolve_hints refl)
+  apply (resolve_hints refl)
+  apply (resolve_hints refl)
+  apply (fold transport_def)
+  apply (transport_relator_rewrite)+
+  apply (unfold transport_def)
+  apply (resolve_hints refl)
+  done
 
 end
-
+end
 
 end
