Transport/Examples/Typedef/Transport_Typedef_Base.thy
@@ -45,15 +45,23 @@ sublocale transport? :
   rewrites "(=\<^bsub>\<lambda>(x :: 'a). x \<in> A\<^esub>) \<equiv> L"
   and "(=\<^bsub>\<top> :: 'b \<Rightarrow> bool\<^esub>) \<equiv> R"
   and "(galois_rel.Galois (=) (=) Rep)\<restriction>\<^bsub>\<lambda>x. x \<in> A\<^esub>\<upharpoonleft>\<^bsub>\<top> :: 'b \<Rightarrow> bool\<^esub> \<equiv>
-    (galois_rel.Galois (=) (=) Rep)\<restriction>\<^bsub>A\<^esub>"
-  using Rep Abs_inverse Rep_inverse
+    (galois_rel.Galois (=) (=) Rep)"
+  using Abs_inverse Rep_inverse
   by (intro transport_eq_restrict_bijection.intro bijection_onI)
-  (auto simp: restrict_right_eq)
+  (auto simp: restrict_right_eq
+    intro!: eq_reflection galois_rel.left_GaloisI Rep
+    elim: galois_rel.left_GaloisE)
 
 interpretation galois L R Abs Rep .
 
-lemma Rep_Left_Galois_self: "Rep y \<^bsub>L\<^esub>\<lessapprox> y"
+lemma Rep_left_Galois_self: "Rep y \<^bsub>L\<^esub>\<lessapprox> y"
   using Rep by (intro left_GaloisI) auto
+
+definition "AR x y \<equiv> x = Rep y"
+
+lemma left_Galois_eq_AR: "left_Galois = AR"
+  unfolding AR_def
+  by (auto intro!: galois_rel.left_GaloisI Rep elim: galois_rel.left_GaloisE)
 
 end
 
