Transport/Examples/Transport_Dep_Fun_Rel.thy
@@ -12,13 +12,17 @@ text \<open>Dependent function relator examples from the paper
 "Transport via Partial Galois Connections and Equivalences" by Kevin Kappelmann.
 Refer to the paper for more details.\<close>
 
-
 context
   includes galois_rel_syntax transport_syntax
   notes
     transport.rel_if_partial_equivalence_rel_equivalence_if_iff_if_partial_equivalence_rel_equivalenceI
-    [per_intro]
+    [rotated, per_intro]
+    transport_Dep_Fun_Rel_no_dep_fun.partial_equivalence_rel_equivalenceI
+    [ML_rattr \<open>Conversion_Util.move_prems_to_front_conv [1] |> CUtil.thm_conv |> K\<close>,
+      ML_rattr \<open>Conversion_Util.move_prems_to_front_conv [2,3] |> CUtil.thm_conv |> K\<close>,
+      per_intro]
 begin
+
 interpretation transport L R l r for L R l r .
 
 abbreviation "Zpos \<equiv> ((=\<^bsub>(\<le>)(0 :: int)\<^esub>) :: int \<Rightarrow> _)"
@@ -26,7 +30,7 @@ abbreviation "Zpos \<equiv> ((=\<^bsub>(\<le>)(0 :: int)\<^esub>) :: int \<Right
 lemma Zpos_per [per_intro]: "(Zpos \<equiv>\<^bsub>PER\<^esub> (=)) nat int"
   by fastforce
 
-lemma sub_parametric [transport_parametric]:
+lemma sub_parametric [transport_in_dom]:
   "([i _ \<Colon> Zpos] \<Rrightarrow> [j _ \<Colon> Zpos | j \<le> i] \<Rrightarrow> Zpos) (-) (-)"
   by fastforce
 
@@ -34,12 +38,12 @@ transport_term nat_sub :: "nat \<Rightarrow> nat \<Rightarrow> nat" where x = "(
   and L = "[i _ \<Colon> Zpos] \<Rrightarrow> [j _ \<Colon> Zpos | j \<le> i] \<Rrightarrow> Zpos"
   and R = "[n _ \<Colon> (=)] \<Rrightarrow> [m _ \<Colon> (=) | m \<le> n] \<Rrightarrow> (=)"
   (*fastforce discharges the remaining side-conditions*)
-  by transport_term_prover fastforce+
+  by (transport_prover) fastforce+
 
+thm nat_sub_app_eq
 text \<open>Note: as of now, @{command transport_term} does not rewrite the
 Galois relator of dependent function relators.\<close>
 thm nat_sub_related'
-thm nat_sub_app_eq
 
 abbreviation "LRel \<equiv> list_all2"
 abbreviation "IARel \<equiv> rel_iarray"
@@ -56,7 +60,7 @@ lemma [per_intro]:
     intro: list.rel_transp list.rel_symp iarray.rel_transp iarray.rel_symp
     elim: iarray.rel_cases)+
 
-lemma [transport_parametric]:
+lemma [transport_in_dom]:
   "([xs _ \<Colon> LRel R] \<Rrightarrow> [i _ \<Colon> (=) | i < length xs] \<Rrightarrow> R) (!) (!)"
   by (fastforce simp: list_all2_lengthD list_all2_nthD2)
 
@@ -66,16 +70,18 @@ begin
 
 interpretation Rper : transport_partial_equivalence_rel_id R
   by unfold_locales per_prover
+
 declare Rper.partial_equivalence_rel_equivalence [per_intro]
 
 transport_term iarray_index where x = "(!) :: 'a list \<Rightarrow> _"
   and L = "([xs _ \<Colon> LRel R] \<Rrightarrow> [i _ \<Colon> (=) | i < length xs] \<Rrightarrow> R)"
   and R = "([xs _ \<Colon> IARel R] \<Rrightarrow> [i _ \<Colon> (=) | i < IArray.length xs] \<Rrightarrow> R)"
-  by transport_term_prover
+  by (transport_prover)
   (*fastforce discharges the remaining side-conditions*)
   (fastforce simp: list_all2_lengthD elim: iarray.rel_cases)+
 
 end
 end
+
 
 end
